added add 'verify' functions

intermediate/Veritas.Intermediate.Store.fsti
@@ -1,13 +1,14 @@
 module Veritas.Intermediate.Store
-open FStar.Integers
 open Veritas.Intermediate.Common
-module U16 = FStar.UInt16
+
 module SA = Veritas.SeqAux
 module R = Veritas.Record
+module BT = Veritas.BinTree
 
 let vstore = Seq.seq (option record)
-let st_index (st:vstore) = SA.seq_index st
+let st_index st = SA.seq_index st
 
+(* get record by slot_id *)
 let get_record (st:vstore) (s:slot_id)
   : option record
   = if s >= Seq.length st then None else Seq.index st s
@@ -16,19 +17,72 @@ let contains_record (st:vstore) (s:slot_id)
   : bool
   = Some? (get_record st s)
 
+let get_key_at (st:vstore) (s:slot_id{contains_record st s})
+  : key
+  = Record?.k (Some?.v (get_record st s))
+
+let get_value_at (st:vstore) (s:slot_id{contains_record st s})
+  : value
+  = Record?.v (Some?.v (get_record st s))
+
+let get_add_method_at (st:vstore) (s:slot_id{contains_record st s})
+  : add_method
+  = Record?.am (Some?.v (get_record st s))
+
+(* get record by key *)
+let lookup_key (st:vstore) (k:key) 
+  : option record
+  = let f ro = if None? ro then false
+               else let Some r = ro in Record?.k r = k in
+    let s = SA.filter f st in
+    if Seq.length s = 0 then None
+    else Seq.index s 0 
+
+let contains_key (st:vstore) (k:key)
+  : bool
+  = Some? (lookup_key st k)
+
+let lemma_lookup_key (st:vstore) (k:key) 
+  : Lemma (requires (contains_key st k))
+          (ensures (Record?.k (Some?.v (lookup_key st k)) = k))
+  = let f ro = if None? ro then false
+               else let Some r = ro in Record?.k r = k in
+    SA.lemma_filter_correct1 f st 0
+
+let lemma_contains_key (st:vstore) (s:slot_id{contains_record st s}) (k:key)
+  : Lemma (requires (get_key_at st s = k))
+          (ensures (contains_key st k))
+  = let f ro = if None? ro then false
+               else let Some r = ro in Record?.k r = k in
+    let sq = SA.filter f st in
+    SA.lemma_filter_exists f st;
+    SA.lemma_filter_correct1 f st 0
+
+let value_of (st:vstore) (k:key{contains_key st k})
+  : R.value_type_of k
+  = lemma_lookup_key st k;
+    Record?.v (Some?.v (lookup_key st k))
+
+let add_method_of (st:vstore) (k:key{contains_key st k})
+  : add_method
+  = Record?.am (Some?.v (lookup_key st k))
+
 let update_record (st:vstore) (s:st_index st) (r:record)
   : vstore
   = Seq.upd st s (Some r)
 
-let update_record_value (st:vstore) (s:st_index st{contains_record st s}) (v:value)
+let update_record_value 
+  (st:vstore) 
+  (s:st_index st{contains_record st s}) 
+  (v:value{R.is_value_of (get_key_at st s) v})
   : vstore
-  = let Some r = get_record st s in
-    update_record st s ({r with record_value = v}) 
+  = let Some (Record k _ am) = get_record st s in
+    update_record st s (Record k v am) 
 
-let add_record (st:vstore) (s:SA.seq_index st) (k:key) (v:value{Veritas.Record.is_value_of k v}) (a:add_method)
+let add_record (st:vstore) (s:st_index st) (k:key) (v:value{R.is_value_of k v}) (am:add_method)
   : vstore
-  = update_record st s (mk_record k v a)
+  = update_record st s (Record k v am)
 
-let evict_record (st:vstore) (s:SA.seq_index st)
+let evict_record (st:vstore) (s:st_index st)
   : vstore
   = Seq.upd st s None
