intermediate/Veritas.Intermediate.Verifier.fst
@@ -1,113 +1,279 @@
 module Veritas.Intermediate.Verifier
-open FStar.Integers
 open Veritas.Intermediate.Common
-module S = Veritas.Intermediate.Store
-module MH = Veritas.MultiSetHash
-open Veritas.Record
-open Veritas.Key
+open Veritas.Intermediate.Store
 
+module R = Veritas.Record
+module K = Veritas.Key
+module H = Veritas.Hash
+module MH = Veritas.MultiSetHash
+module MHD = Veritas.MultiSetHashDomain
+module BT = Veritas.BinTree
+module V = Veritas.Verifier
+
+(* id     : thread id
+   st     : thread local store
+   clock  : current timestamp
+   hadd   : add set hash
+   hevict : evict set hash
+   valid  : has the a Blum add violated the key store invariant? 
+            >> will trigger transition to Failed later *)
 noeq
 type vtls =
   | Failed : vtls
   | Valid :
-    id : thread_id_t ->
-    st : S.vstore ->
+    id : thread_id ->
+    st : vstore ->
     clock : timestamp ->
     hadd : MH.ms_hash_value ->
     hevict : MH.ms_hash_value ->
+    valid : bool ->
     vtls
 
-let update_thread_store (vs:vtls {Valid? vs})
-                        (st:S.vstore)
-                        : vtls =
-  match vs with
-  | Valid id _ clock hadd hevict -> Valid id st clock hadd hevict
+let thread_id_of (vs:vtls {Valid? vs}): thread_id = 
+  Valid?.id vs
 
-let thread_store (vs:vtls { Valid? vs } )
-  : S.vstore
-  = Valid?.st vs
+let thread_store (vs: vtls {Valid? vs}): vstore =
+  Valid?.st vs
+
+let update_thread_store (vs:vtls {Valid? vs}) (st:vstore) : vtls =
+  match vs with
+  | Valid id _ clock hadd hevict valid -> Valid id st clock hadd hevict valid
+
+let thread_clock (vs:vtls {Valid? vs}) = 
+  Valid?.clock vs
+
+let update_thread_clock (vs:vtls {Valid? vs}) (clock:timestamp): vtls = 
+  match vs with
+  | Valid id st _ hadd hevict valid -> Valid id st clock hadd hevict valid
+
+let thread_hadd (vs:vtls {Valid? vs}) = 
+  Valid?.hadd vs
+
+let thread_hevict (vs:vtls {Valid? vs}) = 
+  Valid?.hevict vs
+
+let update_thread_hadd (vs:vtls {Valid? vs}) (hadd: MH.ms_hash_value): vtls = 
+  match vs with
+  | Valid id st clock _ hevict valid -> Valid id st clock hadd hevict valid
+
+let update_thread_hevict (vs:vtls {Valid? vs}) (hevict:MH.ms_hash_value): vtls = 
+  match vs with
+  | Valid id st clock hadd _ valid -> Valid id st clock hadd hevict valid
+
+let thread_valid (vs: vtls {Valid? vs}) =
+  Valid?.valid vs
+
+let update_thread_valid (vs:vtls {Valid? vs}) (valid:bool): vtls = 
+  match vs with
+  | Valid id st clock hadd hevict _ -> Valid id st clock hadd hevict valid
 
 let vget (s:slot_id) (v:data_value) (vs: vtls {Valid? vs}): vtls =
   let st = thread_store vs in
-  (* check if store contains slot s *)
-  if not (S.contains_record st s) then Failed
-  (* check if stored value is v *)
-  else let Some r = S.get_record st s in
-       if not (DVal? r.record_value)
-       then Failed
-       else if to_data_value r.record_value <> v
-       then Failed
+  (* check store contains slot s *)
+  if not (contains_record st s) then Failed
+  (* check stored value is v *)
+  else let v' = get_value_at st s in
+       if not (R.DVal? v') then Failed
+       else if R.to_data_value v' <> v then Failed
        else vs
 
 let vput (s:slot_id) (v:data_value) (vs: vtls {Valid? vs}): vtls =
   let st = thread_store vs in
-  (* check if store contains slot s *)
-  if not (S.contains_record st s) then Failed
-  else update_thread_store vs (S.update_record_value st s (DVal v))
+  (* check store contains slot s *)
+  if not (contains_record st s) then Failed
+  (* check stored key is a data key *)
+  else if not (K.is_data_key (get_key_at st s)) then Failed
+  else update_thread_store vs (update_record_value st s (R.DVal v))
 
-let vaddm (s:slot_id) (r:Veritas.Intermediate.Common.record) (s':slot_id) (vs: vtls {Valid? vs}): vtls =
+let vaddm (s:slot_id) (r:record) (s':slot_id) (vs: vtls {Valid? vs}): vtls =
   let st = thread_store vs in
-  if s > Seq.length st then Failed
-  //let { record_key = k; record_value = v } = r in
-  else let k = r.record_key in
-  let v = r.record_value in
-  (* the store should contain slot s' *)
-  if not (S.contains_record st s') then Failed
-  else 
-    let Some r' = S.get_record st s' in
-    let { 
-          record_key = k';
-          record_value = v';
-          record_add_method = a;
-          record_l_child_in_store = l_in_store;
-          record_r_child_in_store = r_in_store
-        } = r' in 
-    (* k should be a proper desc of k' *)
-    if not (Veritas.BinTree.is_proper_desc k k') then Failed
-    (* the store should not contain slot s *)
-    else if S.contains_record st s then Failed
-    (* the type of v should be consistent with k *)
-    else if not (is_value_of k v) then Failed
-    (* v' should be a merkle value *)
-    else if DVal? v' then Failed 
+  if not (s < Seq.length st) then Failed
+  (* check store contains slot s' *)
+  else if not (contains_record st s') then Failed
+  else
+    let k = Record?.k r in
+    let v = Record?.v r in
+    let k' = get_key_at st s' in
+    let v' = get_value_at st s' in
+    let a' = get_add_method_at st s' in 
+    (* check k is a proper desc of k' *)
+    if not (BT.is_proper_desc k k') then Failed
+    (* check store does not contain slot s *)
+    else if contains_record st s then Failed
+    (* check type of v is consistent with k *)
+    else if not (R.is_value_of k v) then Failed
+    (* check v' is a merkle value *)
+    else if R.DVal? v' then Failed 
     else
-      let v' = to_merkle_value v' in
-      let d = Veritas.BinTree.desc_dir k k' in
-      let dh' = desc_hash_dir v' d in 
-      (* check whether k is already in the store *)
-      if Veritas.BinTree.Left? d && Desc? dh' && l_in_store then Failed
-      else if Veritas.BinTree.Right? d && Desc? dh' && r_in_store then Failed
-      else let h = Veritas.Hash.hashfn v in
+      let v' = R.to_merkle_value v' in
+      let d = BT.desc_dir k k' in
+      let dh' = R.desc_hash_dir v' d in 
+      (* check k is not already in the store
+         >> in lower levels we will check this via 'in_store' fields in records *)
+      if contains_key st k then Failed
+      else let h = H.hashfn v in
       match dh' with
-      | Empty -> if v = init_value k then
-                   let v'_upd = Veritas.Verifier.update_merkle_value v' d k h false in
-                   let st_upd = S.update_record_value st s' (MVal v'_upd) in
-                   let st_upd2 = S.add_record st_upd s k v Veritas.Verifier.MAdd in
-                   update_thread_store vs st_upd2
-                 else Failed
-      | Desc k2 h2 b2 -> if k2 = k then
-                           if h2 = h && b2 = false then
-                             update_thread_store vs (S.add_record st s k v Veritas.Verifier.MAdd)
-                           else Failed
-                         else if v <> init_value k then Failed
-                         else if not (Veritas.BinTree.is_proper_desc k2 k) then Failed
-                         else
-                           let d2 = Veritas.BinTree.desc_dir k2 k in
-                           let mv = to_merkle_value v in
-                           let mv_upd = Veritas.Verifier.update_merkle_value mv d2 k2 h2 b2 in
-                           let v'_upd = Veritas.Verifier.update_merkle_value v' d k h false in
-                           let st_upd = S.update_record_value st s' (MVal  v'_upd) in // need to update s' to say that the child in direction d is present
-                           let st_upd2 = S.add_record st_upd s k (MVal mv_upd) Veritas.Verifier.MAdd in
-                           update_thread_store vs st_upd2
+      | R.Empty -> (* k' has no child in direction d *)
+                (* first add --> init value *)
+                if v <> R.init_value k then Failed
+                else
+                  let v'_upd = V.update_merkle_value v' d k h false in
+                  let st_upd = update_record_value st s' (R.MVal v'_upd) in
+                  let st_upd2 = add_record st_upd s k v V.MAdd in
+                  update_thread_store vs st_upd2
+      | R.Desc k2 h2 b2 -> if k2 = k then
+                          (* k is a child of k' *)
+                          (* check hashes match and k was not evicted to blum *)
+                          if not (h2 = h && b2 = false) then Failed
+                          else update_thread_store vs (add_record st s k v V.MAdd)
+                          (* k is not a child of k' *)
+                          (* first add --> init value *)
+                        else if v <> R.init_value k then Failed
+                        (* check k2 is a proper desc of k *)
+                        else if not (BT.is_proper_desc k2 k) then Failed
+                        else
+                          let d2 = BT.desc_dir k2 k in
+                          let mv = R.to_merkle_value v in
+                          let mv_upd = V.update_merkle_value mv d2 k2 h2 b2 in
+                          let v'_upd = V.update_merkle_value v' d k h false in
+                          let st_upd = update_record_value st s' (R.MVal  v'_upd) in
+                          let st_upd2 = add_record st_upd s k (R.MVal mv_upd) V.MAdd in
+                          update_thread_store vs st_upd2
+
+(* key k is in store and was added using Merkle *)
+let is_instore_madd (st: vstore) (k: key): bool = 
+  contains_key st k && 
+  add_method_of st k = V.MAdd
+
+let has_instore_merkle_desc (st: vstore) (k:key{contains_key st k}): bool = 
+  if K.is_data_key k then false
+  else 
+    let v = R.to_merkle_value (value_of st k) in
+    let ld = R.desc_hash_dir v BT.Left in
+    let rd = R.desc_hash_dir v BT.Right in
+    R.Desc? ld && is_instore_madd st (R.Desc?.k ld) || 
+    R.Desc? rd && is_instore_madd st (R.Desc?.k rd)
+
+let vevictm (s s':slot_id) (vs: vtls {Valid? vs}): vtls = 
+  let st = thread_store vs in
+  (* check store contains s and s' *)
+  if not (contains_record st s && contains_record st s') then Failed
+  else 
+    let k = get_key_at st s in
+    let v = get_value_at st s in
+    let a = get_add_method_at st s in
+    let k' = get_key_at st s' in
+    let v' = get_value_at st s' in
+    let a' = get_add_method_at st s' in
+    (* check k is a proper descendent of k' *)
+    if not (BT.is_proper_desc k k') then Failed
+    (* check k does not have a child in the store *)
+    else if (
+              lemma_contains_key st s k; 
+              has_instore_merkle_desc st k
+            ) then Failed
+    else 
+      let d = BT.desc_dir k k' in
+      let v' = R.to_merkle_value v' in
+      let dh' = R.desc_hash_dir v' d in
+      let h = H.hashfn v in
+      match dh' with
+      | R.Empty -> Failed
+      | R.Desc k2 h2 b2 -> if k2 <> k then Failed
+                        else
+                          let v'_upd = V.update_merkle_value v' d k h false in
+                          let st_upd = evict_record (update_record_value st s' (R.MVal v'_upd)) s in
+                         update_thread_store vs st_upd
+
+let vaddb (s:slot_id) (r:record) (t:timestamp) (j:thread_id) (vs:vtls {Valid? vs}): vtls = 
+  let st = thread_store vs in 
+  if not (s < Seq.length st) then Failed
+  (* epoch of timestamp of last evict *)
+  else 
+    let e = MHD.MkTimestamp?.e t in
+    let k = Record?.k r in
+    let v = Record?.v r in
+    (* check value type consistent with key k *)
+    if not (R.is_value_of k v) then Failed
+    (* check store contains slot s *)
+    else if contains_record st s then Failed
+    else 
+      (* check k is not in the store; update the valid flag accordingly *)
+      let valid = not (contains_key st k) in
+      let vs_upd = update_thread_valid vs (thread_valid vs && valid) in
+      (* update add hash *)
+      let h = thread_hadd vs in
+      let h_upd = MH.ms_hashfn_upd (MHD.MHDom (k,v) t j) h in
+      let vs_upd2 = update_thread_hadd vs_upd h_upd in
+      (* update clock *)
+      let clk = thread_clock vs in
+      let clk_upd = V.max clk (MHD.next t) in
+      let vs_upd3 = update_thread_clock vs_upd2 clk_upd in
+      (* add record to store *)
+      let st_upd = add_record st s k v V.BAdd in
+      update_thread_store vs_upd3 st_upd
+
+let vevictb (s:slot_id) (t:timestamp) (vs:vtls {Valid? vs}): vtls = 
+  let clock = thread_clock vs in
+  let e = MHD.MkTimestamp?.e t in
+  let st = thread_store vs in
+  (* check store contains slot s *)
+  if not (contains_record st s) then Failed
+  else
+    let k = get_key_at st s in
+    let v = get_value_at st s in
+    (* check key at s is not root *)
+    if k = BT.Root then Failed
+    (* check time of evict < current time *)
+    else if not (MHD.ts_lt clock t) then Failed
+    (* check s was added through blum *)  
+    else if get_add_method_at st s <> V.BAdd then Failed
+    (* check k has no children n the store *)
+    else if (
+              lemma_contains_key st s k;
+              has_instore_merkle_desc st k
+            ) then Failed  
+    else 
+      (* update evict hash *)
+      let h = thread_hevict vs in
+      let h_upd = MH.ms_hashfn_upd (MHD.MHDom (k,v) t (thread_id_of vs)) h in
+      let vs_upd = update_thread_hevict vs h_upd in
+      (* update clock *)
+      let vs_upd2 = update_thread_clock vs_upd t in    
+      (* evict record *)
+      let st_upd = evict_record st s in
+      update_thread_store vs_upd2 st_upd
+
+let vevictbm (s s':slot_id) (t:timestamp) (vs:vtls {Valid? vs}): vtls = 
+  let st = thread_store vs in
+  (* check store contains s and s' *)
+  if not (contains_record st s && contains_record st s') then Failed
+  else
+    let k = get_key_at st s in
+    let k' = get_key_at st s' in
+    let v' = get_value_at st s' in
+    (* check k is a proper desc of k' *)
+    if not (BT.is_proper_desc k k') then Failed
+    (* check s was added through merkle *)
+    else if get_add_method_at st s <> V.MAdd then Failed  
+    (* check k has no children in the store *)
+    else if (
+              lemma_contains_key st s k;
+              has_instore_merkle_desc st k 
+            ) then Failed  
+    else
+      let v' = R.to_merkle_value v' in
+      let d = BT.desc_dir k k' in
+      let dh' = R.desc_hash_dir v' d in
+      match dh' with
+      | R.Empty -> Failed
+      | R.Desc k2 h2 b2 -> if k2 <> k || b2 then Failed
+                          else
+                            let v'_upd = V.update_merkle_value v' d k h2 true in
+                            let st_upd = update_record_value st s' (R.MVal v'_upd) in
+                            vevictb s t (update_thread_store vs st_upd)
 
 
-// vevictm
-
-// vaddb
-
-// vevictb
-
-// vevictbm
 
 
 (* Per invariant.md, we will want to prove something like the following for
