intermediate/Veritas.Intermediate.Common.fsti
@@ -1,42 +1,19 @@
 module Veritas.Intermediate.Common
-open FStar.Integers
-
-module U8 = FStar.UInt8
-module U16 = FStar.UInt16
-module U32 = FStar.UInt32
-module U64 = FStar.UInt64
-module U128 = FStar.UInt128
 open Veritas.Record
+
 type slot_id = nat
 
 let key = Veritas.Key.key
-
-val most_significant_bit (k:key) : bool
-
 let value = Veritas.Record.value
-let data_value = Veritas.Record.data_value
-
+let data_value = Veritas.Record.data_value 
 let add_method = Veritas.Verifier.add_method
 
-type record = {
-  record_key:key;
-  record_value:value;
-  record_add_method:add_method;
-  record_l_child_in_store:bool;
-  record_r_child_in_store:bool
-}
+(* KH: too high-level to require value_of_type_k? does this add runtime overhead
+   in extracted code? *)
+type record = 
+  | Record: k:key -> v:value_type_of k -> am:add_method -> record
 
-
-let mk_record k v a : record = {
-  record_key = k;
-  record_value = v;
-  record_add_method = a;
-  record_l_child_in_store = false;
-  record_r_child_in_store = false;
-}
-
-let thread_id_t = nat
-
+let thread_id = Veritas.Verifier.thread_id
 let timestamp = Veritas.MultiSetHashDomain.timestamp
 
 noeq
@@ -57,7 +34,7 @@ type vlog_entry =
   | AddB:    s:slot_id ->
              r:record ->
              t:timestamp ->
-             j:thread_id_t ->
+             j:thread_id ->
              vlog_entry
   | EvictB:  s:slot_id ->
              t:timestamp ->
