intermediate/Veritas.Intermediate.Hash.fsti
@@ -1,6 +1,0 @@
-module Veritas.Intermediate.Hash
-
-val hash_key : eqtype
-val hash : eqtype
-val init (k:hash_key) : hash
-
